\documentclass{article}
\usepackage{graphicx}
\usepackage[left=3.5cm, right = 3.5cm, top=3.5cm, bottom=3.5cm, head=13.6pt]{geometry}
\usepackage[onehalfspacing]{setspace}
\usepackage{amsthm}
\usepackage{amsmath}
\usepackage{amssymb}
\usepackage{mathtools}
\usepackage{float}
\usepackage{algpseudocode}
\usepackage{algorithm}
\usepackage{comment}
\usepackage{csquotes}
\usepackage{enumitem}
\usepackage{stmaryrd}

\title{\vspace{-3.5cm}Advanced Topics in Computer Graphics I - Sheet R10}
\author{Ninian Kaspers, Robin Landsgesell, Julian Stamm}
\date{\today}

\begin{document}

    \maketitle

    \section*{Assignment 2}
    a)
    \begin{equation*}
        p_{HG}(\mu | g) = \frac{1 - g^2}{2} \cdot (1 + g^2 - 2 g \mu)^{-\frac{3}{2}}
    \end{equation*}
    \scalebox{0.84}{\parbox{.5\linewidth}{%
    \begin{align*}
        \mathbb{E}[\mu] &= \int_{-1}^{1} \mu \cdot p_{HG}(\mu | g) d\mu\\
        &= \int_{-1}^{1} \mu \cdot \frac{1 - g^2}{2} \cdot (1 + g^2 - 2 g \mu)^{-\frac{3}{2}} d\mu\\
        &= \frac{1 - g^2}{2} \cdot \int_{-1}^{1} \mu \cdot (1 + g^2 - 2 g \mu)^{-\frac{3}{2}} d\mu\\
        &\text{ substitute } t = 1 + g^2 - 2g \mu \Leftrightarrow \mu = \frac{1 + g^2 - t}{2g} \text{ with } dt = -2g\,d\mu \Leftrightarrow d\mu = \frac{1}{-2g}dt\\
        &= \frac{1 - g^2}{2} \cdot \int_{(1+g)^2}^{(1-g)^2} \frac{1 + g^2 - t}{2g} \cdot t^{-\frac{3}{2}} \cdot \frac{1}{-2g}dt\\
        &= \frac{1 - g^2}{2} \cdot -\frac{1}{4g^2} \cdot \int_{(1+g)^2}^{(1-g)^2} (1 + g^2 - t) \cdot t^{-\frac{3}{2}} dt\\
        &= -\frac{1 - g^2}{8g^2} \cdot \int_{(1+g)^2}^{(1-g)^2} (1 + g^2) t^{-\frac{3}{2}} - t^{-\frac{1}{2}} dt\\
        &= -\frac{1 - g^2}{8g^2} \cdot \int_{(1+g)^2}^{(1-g)^2} (1 + g^2) t^{-\frac{3}{2}} dt - \int_{(1+g)^2}^{(1-g)^2} t^{-\frac{1}{2}} dt\\
        &= -\frac{1 - g^2}{8g^2} \cdot \left[\left( (1 + g^2) \cdot \int_{(1+g)^2}^{(1-g)^2} t^{-\frac{3}{2}} dt \right) - \int_{(1+g)^2}^{(1-g)^2} t^{-\frac{1}{2}} dt \right]\\
        &\text{with } \int t^{-\frac{3}{2}} dt = -2t^{-\frac{1}{2}} \text{ and } \int t^{-\frac{1}{2}} dt = 2t^{\frac{1}{2}}\\
        &= -\frac{1 - g^2}{8g^2} \cdot \left[\left((1 + g^2) \cdot \left[-2t^{-\frac{1}{2}}\right]_{(1+g)^2}^{(1-g)^2} \right) - \left[2t^{\frac{1}{2}}\right]_{(1+g)^2}^{(1-g)^2} \right]\\
        &= -\frac{1 - g^2}{8g^2} \cdot \left[\left( (1 + g^2) \cdot \left[-2((1-g)^2)^{-\frac{1}{2}} + 2((1+g)^2)^{-\frac{1}{2}}\right]\right) - \left[2((1-g)^2)^{\frac{1}{2}} - 2((1+g)^2)^{\frac{1}{2}}\right] \right]\\
        &= -\frac{1 - g^2}{8g^2} \cdot \left[\left( (1 + g^2) \cdot \left[-2((1-g)^2)^{-\frac{1}{2}} + 2((1+g)^2)^{-\frac{1}{2}}\right]\right) - 2((1-g)^2)^{\frac{1}{2}} + 2((1+g)^2)^{\frac{1}{2}} \right]\\
        &= -\frac{1 - g^2}{8g^2} \cdot \left[ (1 + g^2) \cdot \left[-2 \cdot \frac{1}{|1-g|} + 2 \cdot \frac{1}{|1+g|}\right] - 2 \cdot |1-g| + 2 \cdot |1+g|\right]\\
        &\text{for } g \in [-1,1]: 1-g \geq 0 \Rightarrow |1-g|=1-g \text{ and } 1+g \geq 0 \Rightarrow |1+g| = 1+g\\
        &= -\frac{1 - g^2}{8g^2} \cdot \left[ (1 + g^2) \cdot \left[-2 \cdot \frac{1}{1-g} + 2 \cdot \frac{1}{1+g}\right] - 2 \cdot (1-g) + 2 \cdot (1+g)\right]\\
        &= -\frac{1 - g^2}{8g^2} \cdot \left[ (1 + g^2) \cdot \left[\frac{-4g}{1-g^2}\right] + 4g\right]\\
        &= -\frac{1 - g^2}{8g^2} \cdot -\frac{8g^3}{1-g^2}\\
        &= g
    \end{align*}
    }}
        
    b) 
    \begin{itemize}
        \item $g=-1$: a dirac delta in the opposite direction of $\omega_i$, purely back-scattering
        \item $g=0$: isotropic scattering, uniformly distributed on the sphere 
        \item $g=1$: a dirac delta in the same direction of $\omega_i$, purely forward-scattering
    \end{itemize}

\end{document}

